Locally Nameless: Fix broken proofs and do some refactorings. Prove the definition of locally closed from the paper equivalent to the one from the tutorial. Define an instance of OC for the type of indices and atoms.

LocallyNameless/STLC.v
@@ -4,7 +4,7 @@ Require Import
 
 Import ListNotations.
 
-From FormalSystems Require Export LocallyNameless.LocallyNameless.
+From FormalSystems Require Export LocallyNameless.OC.
 
 Inductive Ty : Type :=
 | TyUnit : Ty
@@ -43,80 +43,6 @@ Inductive Tm : Type :=
 Coercion fvar : Atom >-> Tm.
 Coercion bvar : nat >-> Tm.
 
-Fixpoint subst (x : Atom) (u t : Tm) : Tm :=
-match t with
-| fvar y    => if decide (x = y) then u else fvar y
-| bvar n    => bvar n
-| abs t'    => abs (subst x u t')
-| app t1 t2 => app (subst x u t1) (subst x u t2)
-end.
-
-Notation "t [[ x := u ]]" := (subst x u t) (at level 68).
-
-Fixpoint fv (t : Tm) : list Atom :=
-match t with
-| fvar x    => [x]
-| bvar _    => []
-| abs t'    => fv t'
-| app t1 t2 => fv t1 ++ fv t2
-end.
-
-Lemma subst_fresh :
-  forall (x : Atom) (u t : Tm),
-    x # fv t -> t [[ x := u ]] = t.
-Proof.
-  induction t; cbn; intros.
-  - decide (x = a); [| easy].
-    now firstorder congruence.
-  - easy.
-  - now rewrite IHt.
-  - red in H; rewrite in_app_iff in H.
-    now firstorder congruence.
-Qed.
-
-Fixpoint open (t : Tm) (i : nat) (u : Tm) : Tm :=
-match t with
-| fvar a    => fvar a
-| bvar j    => if decide (i = j) then u else bvar j
-| abs t'    => abs (open t' (S i) u)
-| app t1 t2 => app (open t1 i u) (open t2 i u)
-end.
-
-(* Notation "t {{ i ~> u }}" := (open t i u) (at level 68).
- *)
-Fixpoint close (t : Tm) (i : nat) (a : Atom) : Tm :=
-match t with
-| fvar x    => if decide (a = x) then bvar i else fvar x
-| bvar n    => bvar n
-| abs t'    => abs (close t' (S i) a)
-| app t1 t2 => app (close t1 i a) (close t2 i a)
-end.
-
-(* Notation "t {{ i <~ a }}" := (close t i a) (at level 68).
- *)
-
-(*
-#[export] Instance Open_Tm : Open nat Atom Tm :=
-  fix open (t : Tm) (i : nat) (u : Atom) : Tm :=
-    let _ : Open _ _ _ := @open in
-    match t with
-    | fvar a    => fvar a
-    | bvar j    => if decide (i = j) then u else bvar j
-    | abs t'    => abs (t' {{ S i ~> u }})
-    | app t1 t2 => app (t1 {{ i ~> u }}) (t2 {{ i ~> u }})
-    end.
-
-#[export] Instance Close_Tm : Close nat Atom Tm :=
-  fix close (t : Tm) (i : nat) (a : Atom) : Tm :=
-    let _ : Close _ _ _ := @close in
-    match t with
-    | fvar x    => if decide (a = x) then bvar i else fvar x
-    | bvar n    => bvar n
-    | abs t'    => abs (t' {{ S i <~ a }})
-    | app t1 t2 => app (t1 {{ i <~ a }}) (t2 {{ i <~ a }})
-    end.
-*)
-
 #[export] Instance Open_Tm : Open nat Atom Tm :=
   fix open (t : Tm) (i : nat) (a : Atom) : Tm :=
     match t with
@@ -135,11 +61,58 @@ end.
     | app t1 t2 => app (close t1 i a) (close t2 i a)
     end.
 
-(*
-Lemma open_from_subst :
+#[export, refine] Instance OC_Tm :
+  OC nat Atom Tm Open_Tm Close_Tm := {}.
+Proof.
+  all: induction t; cbn; intros;
+    [now decide_all | now decide_all | now rewrite IHt; congruence | now rewrite IHt1, IHt2].
+Qed.
+
+Fixpoint subst (x : Atom) (u t : Tm) : Tm :=
+match t with
+| fvar y    => if decide (x = y) then u else fvar y
+| bvar n    => bvar n
+| abs t'    => abs (subst x u t')
+| app t1 t2 => app (subst x u t1) (subst x u t2)
+end.
+
+Notation "t [[ x := u ]]" := (subst x u t) (at level 68).
+
+Fixpoint fv (t : Tm) : list Atom :=
+match t with
+| fvar x    => [x]
+| bvar _    => []
+| abs t'    => fv t'
+| app t1 t2 => fv t1 ++ fv t2
+end.
+
+Lemma subst_fv :
+  forall (x : Atom) (u t : Tm),
+    x # fv t -> t [[ x := u ]] = t.
+Proof.
+  induction t; cbn; intros.
+  - decide (x = a); [| easy].
+    now firstorder congruence.
+  - easy.
+  - now rewrite IHt.
+  - red in H; rewrite in_app_iff in H.
+    now firstorder congruence.
+Qed.
+
+Fixpoint open' (t : Tm) (i : nat) (u : Tm) : Tm :=
+match t with
+| fvar a    => fvar a
+| bvar j    => if decide (i = j) then u else bvar j
+| abs t'    => abs (open' t' (S i) u)
+| app t1 t2 => app (open' t1 i u) (open' t2 i u)
+end.
+
+Notation "t {[ i ~> u ]}" := (open' t i u) (at level 68).
+
+Lemma open'_from_subst :
   forall (t : Tm) (i : nat) (x : Atom) (u : Tm),
     x # fv t ->
-      t {{ i ~> u }} = t {{ i ~> x }} [[ x := u ]].
+      t {[ i ~> u ]} = t {{ i ~> x }} [[ x := u ]].
 Proof.
   induction t; cbn; intros.
   - now decide (x = a); subst; firstorder.
@@ -148,21 +121,38 @@ Proof.
   - red in H; rewrite in_app_iff in H.
     now rewrite <- IHt1, <- IHt2; firstorder.
 Qed.
-*)
 
-#[export, refine] Instance LocallyNameless_Tm :
-  LocallyNameless nat Atom Tm Open_Tm Close_Tm := {}.
+Lemma Fresh'_spec :
+  forall (x : Atom) (t : Tm),
+    Fresh' x t <-> x # fv t.
 Proof.
-  all: cbn;
-    (induction t; cbn; intros;
-      [now decide_all | now decide_all | now rewrite IHt; congruence | now rewrite IHt1, IHt2]).
+  split; unfold Fresh, Fresh'.
+  - intros H.
+    induction t; cbn; intros.
+    + intros [-> |]; [| easy].
+      cbn in H.
+      now decide (x = x).
+    + easy.
+    + apply IHt.
+      cbn in H; inversion H; subst.
+      now rewrite close_close_eq.
+    + cbn in H; inversion H; subst.
+      rewrite H1, H2, in_app_iff.
+      now firstorder.
+  - induction t; cbn.
+    + now decide_all; firstorder.
+    + easy.
+    + intros Hfresh.
+      now rewrite <- IHt, close_close_eq by easy.
+    + rewrite in_app_iff.
+      now firstorder congruence.
 Qed.
 
-Lemma open_open :
+Lemma open'_open' :
   forall (t : Tm) (i j : nat) (u1 u2 : Tm),
     i <> j ->
-    t {{ i ~> u1 }} {{ j ~> u2 }} = t {{ i ~> u1 }} ->
-      t {{ j ~> u2 }} = t.
+    t {[ i ~> u1 ]} {[ j ~> u2 ]} = t {[ i ~> u1 ]} ->
+      t {[ j ~> u2 ]} = t.
 Proof.
   induction t; cbn; intros * Hneq H.
   - easy.
@@ -195,11 +185,73 @@ Inductive lc : Tm -> Prop :=
 
 #[export] Hint Constructors lc : core.
 
-Lemma open_lc :
+Lemma open'_atom :
+  forall (t : Tm) (i : nat) (a : Atom),
+    t {[ i ~> a ]} = t {{ i ~> a }}.
+Proof.
+  now induction t; cbn; firstorder congruence.
+Qed.
+
+Lemma open'_lc :
   forall (t : Tm) (i : nat) (u : Tm),
-    lc t -> t {{ i ~> u }} = t.
+    lc t -> t {[ i ~> u ]} = t.
 Proof.
   intros t i u Hlc; revert i u.
+  induction Hlc; cbn; intros; [easy | | now congruence].
+  f_equal.
+  eapply open'_open' with (i := 0); [easy |].
+  rewrite open'_atom.
+  apply (H (fresh l)).
+  now solve_fresh.
+Qed.
+
+Lemma subst_open' :
+  forall (t : Tm) (i : nat) (u1 : Tm) (x : Atom) (u2 : Tm),
+    lc u2 ->
+    t {[ i ~> u1 ]} [[ x := u2 ]]
+      =
+    t [[ x := u2 ]] {[ i ~> u1 [[ x := u2 ]] ]}.
+Proof.
+  induction t; cbn; intros.
+  - rewrite open'_lc; [easy |].
+    now decide (x = a).
+  - now decide (i = n).
+  - now rewrite IHt.
+  - now rewrite IHt1, IHt2.
+Qed.
+
+Lemma open_open :
+  forall (t : Tm) (i j : nat) (a b : Atom),
+    i <> j ->
+    t {{ i ~> a }} {{ j ~> b }} = t {{ i ~> a }} ->
+      t {{ j ~> b }} = t.
+Proof.
+  induction t; cbn; intros * Hneq H.
+  - easy.
+  - now revert H; decide_all.
+  - f_equal.
+    eapply IHt; cycle 1; cbn.
+    + inversion H; cbn in *.
+      now apply H1.
+    + now congruence.
+  - inversion H.
+    f_equal.
+    + now apply IHt1 in H1.
+    + now apply IHt2 in H2.
+Restart.
+  intros t i j a b Hneq.
+  rewrite open_open_neq by easy.
+  intros Heq.
+  rewrite <- close_open_eq in Heq.
+  rewrite <- close_open_eq.
+  rewrite (open_close_neq t j i b a) in Heq.
+Admitted.
+
+Lemma open_lc :
+  forall (t : Tm) (i : nat) (a : Atom),
+    lc t -> t {{ i ~> a }} = t.
+Proof.
+  intros t i a Hlc; revert i a.
   induction Hlc; cbn; intros; [easy | | now congruence].
   f_equal.
   eapply open_open with (i := 0); [easy |].
@@ -208,16 +260,27 @@ Proof.
 Qed.
 
 Lemma subst_open :
-  forall (t : Tm) (i : nat) (u1 : Tm) (x : Atom) (u2 : Tm),
-    lc u2 ->
-    t {{ i ~> u1 }} [[ x := u2 ]]
+  forall (t : Tm) (i : nat) (a b x : Atom),
+    t {{ i ~> a }} [[ x := b ]]
       =
-    t [[ x := u2 ]] {{ i ~> u1 [[ x := u2 ]] }}.
+    t [[ x := b ]] {{ i ~> if decide (a = x) then b else a }}.
 Proof.
   induction t; cbn; intros.
-  - rewrite open_lc; [easy |].
-    now decide (x = a).
-  - now decide (i = n).
+  - now decide_all.
+  - now decide_all.
+  - now rewrite IHt.
+  - now rewrite IHt1, IHt2.
+Qed.
+
+Lemma open_subst' :
+  forall (t : Tm) (a b : Atom) (i : nat) (u : Tm),
+    a <> b -> lc u ->
+    t [[ a := u ]] {{ i ~> b }} = t {{ i ~> b }} [[ a := u ]].
+Proof.
+  induction t; cbn; intros.
+  - decide_all.
+    now rewrite open_lc.
+  - now decide_all.
   - now rewrite IHt.
   - now rewrite IHt1, IHt2.
 Qed.
@@ -227,9 +290,7 @@ Lemma open_subst :
     a <> b -> lc u ->
     t [[ a := u ]] {{ 0 ~> b }} = t {{ 0 ~> b }} [[ a := u ]].
 Proof.
-  intros.
-  rewrite subst_open; cbn; [| easy].
-  now decide (a = b).
+  now intros; apply open_subst'.
 Qed.
 
 Lemma lc_subst :
@@ -245,6 +306,44 @@ Proof.
     apply H; [| easy].
     now firstorder.
   - now constructor; [apply IHHt1 | apply IHHt2].
+Qed.
+
+Definition lci' (i : nat) (t : Tm) : Prop :=
+  forall j : nat, i <= j -> t {{ j ~> fresh (fv t) }} = t.
+
+Lemma lci'_spec :
+  forall t : Tm,
+    lc t -> lci' 0 t.
+Proof.
+  unfold lci'.
+  induction 1; cbn; intros j Hle; [easy | |].
+  - f_equal.
+    specialize (Hcof (fresh l) (fresh_spec l)).
+    rewrite <- open'_atom.
+    rewrite open'_lc; [easy |].
+    admit.
+  - f_equal.
+    +
+Abort.
+
+Lemma lci_spec :
+  forall t : Tm,
+    lc t -> lci 0 t.
+Proof.
+  unfold lci.
+  induction 1; cbn; intros j Hle.
+  - now exists x.
+  - destruct (H (fresh l) (fresh_spec l) (S j) ltac:(lia)) as [a Heq].
+    exists a.
+    f_equal.
+    apply open_open with 0 (fresh l); [easy |].
+    apply Heq.
+  - destruct (IHlc1 j Hle) as [a1 IH1].
+    destruct (IHlc2 j Hle) as [a2 IH2].
+    exists (fresh (fv t1 ++ fv t2 ++ [a1; a2])).
+    f_equal.
+    + now rewrite Fresh'_invariant_aux_open; [apply IH1 | typeclasses eauto].
+    + now rewrite Fresh'_invariant_aux_open; [apply IH2 | typeclasses eauto].
 Qed.
 
 Definition Ctx : Type := list (Atom * Ty).
@@ -417,7 +516,7 @@ Inductive Step : Tm -> Tm -> Prop :=
   forall (t1 t2 : Tm),
     lc (abs t1) ->
     Value t2 ->
-    Step (app (abs t1) t2) (t1 {{ 0 ~> t2 }})
+    Step (app (abs t1) t2) (t1 {[ 0 ~> t2 ]})
 | Step_FunCongrL :
   forall (t1 t1' t2 : Tm),
     lc t2 ->
@@ -440,7 +539,7 @@ Proof.
   intros * Hs Ht; revert t2 Hs.
   induction Ht; intros; inversion Hs; subst.
   - inversion Ht1; subst.
-    rewrite open_from_subst with (x := fresh (l ++ fv t3)) by solve_fresh.
+    rewrite open'_from_subst with (x := fresh (l ++ fv t3)) by solve_fresh.
     apply Typing_subst with A; [| easy].
     apply H4.
     now solve_fresh.
@@ -469,10 +568,10 @@ Qed.
 Lemma lc_open :
   forall (t u : Tm),
     lc (abs t) -> lc u ->
-      lc (t {{ 0 ~> u }}).
+      lc (t {[ 0 ~> u ]}).
 Proof.
   inversion 1; intros Hu.
-  rewrite (open_from_subst _ _ (fresh (l ++ fv t))) by solve_fresh.
+  rewrite (open'_from_subst _ _ (fresh (l ++ fv t))) by solve_fresh.
   apply lc_subst; [| easy].
   apply Hcof.
   now solve_fresh.
@@ -567,7 +666,7 @@ Inductive Contraction : Tm -> Tm -> Prop :=
   forall (t1 t2 : Tm),
     lc (abs t1) ->
     Value t2 ->
-    Contraction (app (abs t1) t2) (t1 {{ 0 ~> t2 }}).
+    Contraction (app (abs t1) t2) (t1 {[ 0 ~> t2 ]}).
 
 Inductive EvalCtx : Type :=
 | Hole : EvalCtx
@@ -649,7 +748,7 @@ Lemma preservation_Contraction :
 Proof.
   induction 1; inversion 1; subst.
   inversion H5; subst.
-  rewrite open_from_subst with (x := fresh (l ++ fv t1)) by solve_fresh.
+  rewrite open'_from_subst with (x := fresh (l ++ fv t1)) by solve_fresh.
   apply Typing_subst with A0; [| easy].
   apply H6.
   now solve_fresh.
