LocallyNameless/OC.v
@@ -1,0 +1,156 @@
+From FormalSystems Require Export LocallyNameless.Atom.
+
+Class Open (Index Atom Term : Type) : Type :=
+  open : Term -> Index -> Atom -> Term.
+
+Class Close (Index Atom Term : Type) : Type :=
+  close : Term -> Index -> Atom -> Term.
+
+Arguments open Index Atom Term Open !_ _ _.
+Arguments close Index Atom Term Close !_ _ _.
+
+Notation "t {{ i ~> a }}" := (open t i a) (at level 68).
+Notation "t {{ i <~ a }}" := (close t i a) (at level 68).
+
+Class OC
+  (Index Atom Term : Type)
+  (OCO : Open Index Atom Term)
+  (OCCC : Close Index Atom Term) : Type :=
+{
+  OC_isAtom :: isAtom Atom;
+  OC_Decidable_eq_Index :: forall i j : Index, Decidable (i = j);
+  open_open_eq : (* OC 1 *)
+    forall (t : Term) (i : Index) (a b : Atom),
+      t {{ i ~> a }} {{ i ~> b }} = t {{ i ~> a }};
+  close_close_eq : (* OC 2 *)
+    forall (t : Term) (i j : Index) (a : Atom),
+      t {{ i <~ a }} {{ j <~ a }} = t {{ i <~ a }};
+  open_close_eq : (* OC 3 *)
+    forall (t : Term) (i : Index) (a : Atom),
+      t {{ i ~> a }} {{ i <~ a }} = t {{ i <~ a }};
+  close_open_eq : (* OC 4 *)
+    forall (t : Term) (i : Index) (a : Atom),
+      t {{ i <~ a }} {{ i ~> a }} = t {{ i ~> a }};
+  open_open_neq : (* OC 5 *)
+    forall (t : Term) (i j : Index) (a b : Atom),
+      i <> j ->
+        t {{ i ~> a }} {{ j ~> b }} = t {{ j ~> b }} {{ i ~> a }};
+  close_close_neq : (* OC 6 *)
+    forall (t : Term) (i j : Index) (a b : Atom),
+      a <> b ->
+        t {{ i <~ a }} {{ j <~ b }} = t {{ j <~ b }} {{ i <~ a }};
+  open_close_neq : (* OC 7 *)
+    forall (t : Term) (i j : Index) (a b : Atom),
+      i <> j -> a <> b ->
+        t {{ i ~> a }} {{ j <~ b }} = t {{ j <~ b }} {{ i ~> a }};
+  open_close_open : (* OC 8 *)
+    forall (t : Term) (i j : Index) (a b : Atom),
+      t {{ i ~> a }} {{ j <~ a }} {{ j ~> b }}
+        =
+      t {{ j ~> b }} {{ i <~ a }} {{ i ~> b }};
+  close_open_close : (* OC 9 *)
+    forall (t : Term) (i j : Index) (a b : Atom),
+      t {{ i <~ a }} {{ i ~> b }} {{ j <~ b }}
+        =
+      t {{ j <~ b }} {{ i ~> a }} {{ j <~ a }}
+}.
+
+(** ** OC set of indices and atoms *)
+
+Section IA.
+
+Context
+  {Index Atom : Type}
+  {Decidable_eq_Index : forall i j : Index, Decidable (i = j)}
+  {isAtom_Atom : isAtom Atom}.
+
+Instance Open_IA : Open Index Atom (Index + Atom) :=
+  fun (ia : Index + Atom) (i : Index) (a : Atom) =>
+    match ia with
+    | inl j => if decide (i = j) then inr a else inl j
+    | inr x => inr x
+    end.
+
+Instance Close_IA : Close Index Atom (Index + Atom) :=
+  fun (ia : Index + Atom) (i : Index) (a : Atom) =>
+    match ia with
+    | inl j => inl j
+    | inr x => if decide (a = x) then inl i else inr x
+    end.
+
+#[refine] Instance OC_IA : OC Index Atom (Index + Atom) Open_IA Close_IA := {}.
+Proof.
+  all: intros [j | x] *; cbn; now decide_all.
+Qed.
+
+End IA.
+
+(** ** Freshness from the paper *)
+
+Section Fresh'_lemmas.
+
+Context
+  (Index Atom Term : Type)
+  (Open_Term : Open Index Atom Term)
+  (Close_Term : Close Index Atom Term)
+  (OC_Term : OC Index Atom Term Open_Term Close_Term).
+
+(* Lemma 2.4 from the paper *)
+Lemma Fresh'_invariant_aux :
+  forall (t : Term) (i j : Index) (a : Atom),
+    t {{ i <~ a }} = t <-> t {{ j <~ a }} = t.
+Proof.
+  now split; intros [= <-]; rewrite close_close_eq.
+Qed.
+
+Lemma Fresh'_invariant_aux' :
+  forall (t : Term) (i : Index) (a : Atom),
+    t {{ i <~ a }} = t <-> forall j : Index, t {{ j <~ a }} = t.
+Proof.
+  split; [| easy].
+  now intros [= <-] j; rewrite close_close_eq.
+Qed.
+
+Lemma Fresh'_invariant_aux_open :
+  forall (t : Term) (i : Index) (a b : Atom),
+    t {{ i ~> a }} = t <-> t {{ i ~> b }} = t.
+Proof.
+  now split; intros [= <-]; rewrite open_open_eq.
+Qed.
+
+End Fresh'_lemmas.
+
+Section Fresh'.
+
+Context
+  {Atom Term : Type}
+  {Open_Term : Open nat Atom Term}
+  {Close_Term : Close nat Atom Term}
+  {OC_Term : OC nat Atom Term Open_Term Close_Term}.
+
+Definition Fresh' (a : Atom) (t : Term) : Prop :=
+  t {{ 0 <~ a }} = t.
+
+Lemma Fresh'_invariant :
+  forall (t : Term) (i : nat) (a : Atom),
+    Fresh' a t <-> t {{ i <~ a }} = t.
+Proof.
+  intros; unfold Fresh'.
+  now rapply Fresh'_invariant_aux.
+Qed.
+
+End Fresh'.
+
+Section lci.
+
+Context
+  {Atom Term : Type}
+  {Open_Term : Open nat Atom Term}
+  {Close_Term : Close nat Atom Term}
+  {OC_Term : OC nat Atom Term Open_Term Close_Term}.
+
+Definition lci (i : nat) (t : Term) : Prop :=
+  forall j : nat, i <= j -> exists a : Atom, t {{ j ~> a }} = t.
+
+End lci.
+
